making reduction/completeness compile again rewriting/confluence for arbitrary pttdom (classes still broken, though)

coq/reduction.v
@@ -9,30 +9,29 @@ Unset Printing Implicit Defensive.
 Set Bullet Behavior "Strict Subproofs". 
 
 Section s.
-Variable A: Type.
-Notation test := (test (tm_pttdom A)). 
-Notation term := (term A).
-Notation graph := (graph test term).
-Notation graph2 := (graph2 test term).
-Notation step := (@step A).
-Notation steps := (@steps A).
+Variable X: pttdom.
+Notation test := (test X). 
+Notation graph := (graph test (car (setoid_of_ops (ops X)))).
+Notation graph2 := (graph2 test (car (setoid_of_ops (ops X)))).
+Notation step := (@step X).
+Notation steps := (@steps X).
 
 
 (* algebraic operations preserve rewriting steps *)
 
 Lemma step_to_steps f:
-  Proper (iso2 ==> iso2) f -> Proper (step ==> steps) f -> Proper (steps ==> steps) f.
+  Proper (iso2prop ==> iso2prop) f -> Proper (step ==> steps) f -> Proper (steps ==> steps) f.
 Proof.
   intros If Sf G G' S.
   induction S as [G G' I|G G' F H' I S Ss IH].
-  - by apply iso_step, If.
-  - etransitivity. apply iso_step, If, I.
+  - by apply isop_step, If.
+  - etransitivity. apply isop_step, If. exists. apply I.
     etransitivity. apply Sf, S. apply IH. 
 Qed.
 
 Instance cnv_steps: Proper (steps ==> steps) (@cnv _).
 Proof.
-  apply step_to_steps. by apply cnv_eqv.
+  apply step_to_steps. simpl. by apply cnv_eqv.
   move=>F G S. eapply one_step. destruct S.
   * apply (@step_v0 _ (point G output input) alpha).
   * apply (@step_v1 _ (point G output input) x u alpha).
@@ -55,7 +54,7 @@ Qed.
 Lemma dot_steps_l G G' H: steps G G' -> steps (G·H) (G'·H).
 Proof.
   apply (step_to_steps (f:=fun G => G·H)) => {G G'}.
-  - move=> ?? E. apply dot_eqv=>//. reflexivity. 
+  - move=> ?? E. apply dot_eqv=>//. 
   - move => G G' GG'. etransitivity. (* apply: (@steps_merge G') => //=. *)
     (* + rewrite /admissible_l/=. by rewrite !inE eqxx. *)
     (* + by rewrite /replace_ioL/= eqxx.  *)
@@ -76,7 +75,7 @@ Qed.
 Lemma par_steps_l G G' H: steps G G' -> steps (G∥H) (G'∥H).
 Proof.
   apply (step_to_steps (f:=fun G => (G∥H)))  => {G G'}. 
-  - move => G G' I. apply par_eqv=>//. reflexivity.
+  - move => G G' I. apply par_eqv=>//. 
   - move => G G' step_G_G'. 
     (* etransitivity. apply: (@steps_merge G') => //=. *)
     (* + by rewrite /admissible_l/= !inE !eqxx. *)
@@ -97,10 +96,34 @@ Proof.
 Qed.
 
 
+End s.
+
+Section s'.
+Variable A: Type.
+Notation term := (term A).  
+Notation nf_term := (nf_term A).  
+Notation test := (test (tm_pttdom A)). 
+Notation graph := (graph test term).
+Notation graph2 := (graph2 test term).
+Notation step := (@step (tm_pttdom A)).
+Notation steps := (@steps (tm_pttdom A)).
+
+
+(* TODO: get rid of this hack... *)
+Canonical Structure tm_bisetoid :=
+  @BiSetoid (tm_setoid A) (@eqv' (tm_pttdom A))
+            (@eqv'_sym (tm_pttdom A))
+            (@eqv10 (tm_pttdom A)) (@eqv01 (tm_pttdom A)) (@eqv11 (tm_pttdom A)).
+(* we would be slightly happier with the following declaration, but Eval hnf does not simplify enough... *)
+(* Canonical Structure tm_bisetoid := Eval hnf in pttdom_bisetoid (tm_pttdom A). *)
+(* following command should work 
+   Check erefl: tm_setoid A = setoid_of_bisetoid _.  
+ *)
+
 (* graphs of terms and normal forms *)
 Definition graph_of_term: term -> graph2 := eval (fun a => g2_var _ (tm_var a)). 
 
-Definition graph_of_nf_term (t: nf_term A): graph2 :=
+Definition graph_of_nf_term (t: nf_term): graph2 :=
   match t with
   | nf_test a => point (unit_graph _ a) tt tt
   | nf_conn a u b => point (edge_graph a u b) false true
@@ -109,30 +132,30 @@ Definition graph_of_nf_term (t: nf_term A): graph2 :=
 
 (* Some of these isomorphism lemma could be slight generalisations of lemmas
    used to get the pttdom laws on graph2 *)
-Lemma ldotunit (G: graph2) a: G · point (unit_graph _ a) tt tt ≃2 G [tst output <- a].
+Lemma ldotunit (G: graph2) a: G · point (unit_graph _ a) tt tt ≃2p G [tst output <- a].
 Admitted.
 
-Lemma lunitdot (G: graph2) a: point (unit_graph _ a) tt tt · G ≃2 G [tst input <- a].
+Lemma lunitdot (G: graph2) a: point (unit_graph _ a) tt tt · G ≃2p G [tst input <- a].
 Admitted.
 
 Lemma lparunitunit (a b: test):
   point (unit_graph term a) tt tt ∥ point (unit_graph _ b) tt tt
-  ≃2 point (unit_graph _ [a·b]) tt tt.
+  ≃2p point (unit_graph _ [a·b]) tt tt.
 Admitted.
 
 Lemma lparedgeunit (u: term) (a b c: test):
   point (edge_graph a u b) false true ∥ point (unit_graph _ c) tt tt
-  ≃2 point (unit_graph _ [c∥a·u·b]) tt tt.
+  ≃2p point (unit_graph _ [c∥a·u·b]) tt tt.
 Admitted.
        
 Lemma add_test_point (a c: test):
   point (unit_graph term a) tt tt [tst tt <- c]
-  ≃2 point (unit_graph _ [a·c]) tt tt.
+  ≃2p point (unit_graph _ [a·c]) tt tt.
 Admitted.                       (* could be inlined for now *)
 
 Lemma add_test_edge (x: bool) (u: term) (a b c: test):
   point (edge_graph a u b) false true [tst x <- c]
-  ≃2 point (edge_graph (if x then a else [c·a]) u (if x then [b·c] else b)) false true.
+  ≃2p point (edge_graph (if x then a else [c·a]) u (if x then [b·c] else b)) false true.
 Admitted.
 
 (* reduction lemma *)
@@ -142,19 +165,19 @@ Proof.
   - etransitivity. apply dot_steps; [apply IHu1|apply IHu2].
     case (nf u1)=>[a|a u b];
     case (nf u2)=>[c|c v d]=>/=.
-    * apply iso_step.
+    * apply isop_step.
       rewrite ldotunit. simpl.
       apply add_test_point. 
-    * apply iso_step.
+    * apply isop_step.
       rewrite lunitdot. simpl.
       apply add_test_edge. 
-    * apply iso_step.
-      setoid_rewrite ldotunit. simpl.
+    * apply isop_step.
+      rewrite ldotunit. simpl.
       apply add_test_edge. 
-    * etransitivity. apply iso_step.
+    * etransitivity. apply isop_step.
       2: etransitivity.
       2: apply one_step, (step_v2 (G:=point (two_graph _ a d) false true) false true u [b·c] v).
-      2: apply iso_step.
+      2: apply isop_step.
       (* 2: liso_step (bij_sym unit_option_void)=>/=. *)
       (* 2: liso bij_id bij_id (fun _ => false)=>//= _; by rewrite !dotA. *)
       (* liso_step merge43=>/=.  *)
@@ -168,21 +191,21 @@ Proof.
   - etransitivity. apply par_steps; [apply IHu1|apply IHu2].
     case (nf u1)=>[a|a u b];
     case (nf u2)=>[c|c v d]=>/=.
-    * apply iso_step. apply lparunitunit.
-    * apply iso_step. rewrite parC. apply lparedgeunit.
-    * apply iso_step. apply lparedgeunit.
-    * etransitivity. apply iso_step.
+    * apply isop_step. apply lparunitunit.
+    * apply isop_step. rewrite parC. apply lparedgeunit.
+    * apply isop_step. apply lparedgeunit.
+    * etransitivity. apply isop_step.
       2: etransitivity.
       2: apply one_step, (step_e2 (G:=point (two_graph _ [a·c] [b·d]) false true) false true u v).
       admit.
-      apply iso_step.
+      apply isop_step.
       (* liso_step (bij_sym unit_option_void)=>/=.  *)
       (* liso bij_id bij_id (fun _ => false)=>//. *)
       admit.
       
   - etransitivity. apply cnv_steps, IHu. 
     case (nf u)=>[a|a v b]=>//=.
-    apply iso_step.
+    apply isop_step.
     (* rewrite /lcnv/=. liso bool_swap bij_id (fun _ => true)=>//=. *)
     (*   by case. *)
     (*   move=>_. apply cnvI. *)
@@ -200,5 +223,4 @@ Proof.
     (* apply dotC.  *)
 Admitted.
 
-End s.
-
+End s'.
